cava/Cava/Lib/BitVectorOps.v
@@ -24,8 +24,8 @@ Export MonadNotation.
 Open Scope monad_scope.
 
 Require Import Cava.Cava.
-Require Import Cava.Core.CavaClass.
-Require Import Cava.Lib.Combinators.
+Require Import Cava.Acorn.CavaClass.
+Require Import Cava.Acorn.Combinators.
 
 Section WithCava.
   Context {signal} `{Cava signal}.
