silveroak-opentitan/aes/Acorn/AddRoundKeyNetlist.v
@@ -21,9 +21,6 @@ Import ListNotations VectorNotations.
 
 Require Import Cava.Cava.
 Require Import Cava.Acorn.Acorn.
-Require Import AesSpec.AES256.
-Require Import AesSpec.Tests.Common.
-Require Import AesSpec.Tests.TestVectors.
 Require Import AcornAes.AddRoundKeyCircuit.
 Require Import AcornAes.Pkg.
 Local Open Scope vector_scope.
@@ -39,63 +36,18 @@ Definition aes_add_round_key_Interface :=
   [mkPort "data_o" (Vec (Vec (Vec Bit 8) 4) 4)]
   [].
 
-Definition aes_add_round_key_Netlist :=
-  makeCircuitNetlist aes_add_round_key_Interface
-                     (Comb (fun '(k,st) => aes_add_round_key k st)).
+Definition aes_add_round_key_Netlist
+  := makeNetlist aes_add_round_key_Interface (fun '(key_i, data_i) => aes_add_round_key key_i data_i).
 
-(* Test bench checking that for a single step, the circuit and Coq semantics
-   return the same result *)
-Section SimpleTest.
-  Definition aes_add_round_key_simple_inputs
-    : list _ := [(fromNatVec test_key, fromNatVec test_state)].
+Local Open Scope list_scope.
 
-  (* Compute the expected outputs from the Coq/Cava semantics. *)
-  Definition aes_add_round_key_simple_expected_outputs : seqType (Vec (Vec (Vec Bit 8) 4) 4)
-    := simulate (Comb (fun '(key_i, data_i) => aes_add_round_key key_i data_i))
-                aes_add_round_key_simple_inputs.
-End SimpleTest.
-
-(* Test bench checking against full FIPS AES-256 encryption test vector *)
-Section FIPSEncryptTests.
-  Definition aes_add_round_key_enc_tb_inputs :=
-    Eval vm_compute in
-      (combine (map from_flat (round_ksch fips_c3_forward))
-               (map from_flat (get_state_inputs AddRoundKey fips_c3_forward))).
-
-  Definition aes_add_round_key_enc_expected_outputs :=
-    Eval vm_compute in
-      (map from_flat (get_state_outputs AddRoundKey fips_c3_forward)).
-End FIPSEncryptTests.
-
-(* Test bench checking against full FIPS AES-256 decryption test vector (for
-   equivalent inverse cipher) *)
-Section FIPSDecryptTests.
-  Definition aes_add_round_key_dec_tb_inputs :=
-    Eval vm_compute in
-      (combine (map from_flat (round_ksch fips_c3_equivalent_inverse))
-               (map from_flat (get_state_inputs AddRoundKey fips_c3_equivalent_inverse))).
-
-  Definition aes_add_round_key_dec_expected_outputs :=
-    Eval vm_compute in
-      (map from_flat (get_state_outputs AddRoundKey fips_c3_equivalent_inverse)).
-End FIPSDecryptTests.
-
-(* Concatenate inputs from all tests *)
-Definition aes_add_round_key_tb_all_inputs :=
-  Eval vm_compute in
-    (aes_add_round_key_simple_inputs
-       ++ aes_add_round_key_enc_tb_inputs
-       ++ aes_add_round_key_dec_tb_inputs)%list.
-
-(* Concatenate expected outputs from all tests *)
-Definition aes_add_round_key_tb_all_expected_outputs :=
-  Eval vm_compute in
-    (aes_add_round_key_simple_expected_outputs
-       ++ aes_add_round_key_enc_expected_outputs
-       ++ aes_add_round_key_dec_expected_outputs)%list.
+(* Compute the expected outputs from the Coq/Cava semantics. *)
+Definition aes_add_round_key_expected_outputs : seqType (Vec (Vec (Vec Bit 8) 4) 4)
+  := multistep (Comb (fun '(key_i, data_i) => aes_add_round_key key_i data_i))
+               [(fromNatVec test_key, fromNatVec test_state)].
 
 Definition aes_add_round_key_tb :=
   testBench "aes_add_round_key_tb"
             aes_add_round_key_Interface
-            aes_add_round_key_tb_all_inputs
-            aes_add_round_key_tb_all_expected_outputs.
+            [(fromNatVec test_key, fromNatVec test_state)]
+            aes_add_round_key_expected_outputs.
