silveroak-opentitan/aes/Acorn/CipherControlNetlist.v
@@ -57,9 +57,9 @@ Definition aes_key_expand_Interface :=
    ; mkPort "clear_i" Bit
    ; mkPort "round_i" (Vec Bit 4)
    ; mkPort "key_len_i" (Vec Bit 3)
-   ; mkPort "key_i" keypair
+   ; mkPort "key_i" key
    ]
-   [ mkPort "key_o" keypair ]
+   [ mkPort "key_o" key ]
    [].
 
 Definition aes_key_expand :
@@ -101,8 +101,7 @@ Definition aes_cipher_core_Interface :=
 
   ; mkPort "prng_data_i" state
   ; mkPort "state_init_i" state
-  ; mkPort "key_init_i" keypair
-
+  ; mkPort "key_init_i" key
 
   ]
   [ mkPort "in_ready_o" Bit
@@ -111,7 +110,6 @@ Definition aes_cipher_core_Interface :=
   ; mkPort "dec_key_gen_o" Bit
   ; mkPort "key_clear_o" Bit
   ; mkPort "data_out_clear_o" Bit
-
   ; mkPort "state_o" state
   ]
   [].
@@ -120,26 +118,6 @@ Definition cipher_loop := CipherCircuit.cipher_loop
   (round_index:=round_index)
   aes_sub_bytes' aes_shift_rows' aes_mix_columns' aes_add_round_key
   inv_mix_columns_key.
-
-Definition aes_cipher_loop_Interface :=
-  sequentialInterface "aes_cipher_loop"
-  "clk_i" PositiveEdge
-  "rst_ni" NegativeEdge
-  [ mkPort "op_i" Bit
-  ; mkPort "num_rounds" round_index
-  ; mkPort "round_0" round_index
-  ; mkPort "curr_round" round_index
-  ; mkPort "key1_i" key
-  ; mkPort "state_i" state
-  ; mkPort "key2_i" key
-  ]
-  [ mkPort "state_o" state
-  ]
-  [].
-
-Definition aes_cipher_loop_Netlist :=
-  makeCircuitNetlist aes_cipher_loop_Interface cipher_loop.
-
 Definition aes_cipher_core := CipherControlCircuit.aes_cipher_core
   aes_key_expand cipher_loop.
 
