tests/DoubleCountBy/DoubleCountBy.v
@@ -111,23 +111,23 @@ Definition b24 := N2Bv_sized 8 24.
 Definition b250 := N2Bv_sized 8 250.
 Definition b251 := N2Bv_sized 8 251.
 
-Goal (simulate
+Goal (multistep
         (Comb addC)
         [(b14,b0); (b7,b14); (b3,b4); (b24,b250)]
       = [(b14,false);(b21,false);(b7,false);(b18,true)]).
 Proof. vm_compute. reflexivity. Qed.
 
-Goal (simulate
+Goal (multistep
         (Comb incrN)
         [b14; b7; b3; b250] = [b15;b8;b4;b251]).
 Proof. vm_compute. reflexivity. Qed.
 
-Goal (simulate
+Goal (multistep
         count_by
         [b14; b7; b3; b250] = [false;false;false;true]).
 Proof. vm_compute. reflexivity. Qed.
 
-Goal (simulate
+Goal (multistep
         double_count_by
         [b14; b7; b3; b250]
       = [b0;b0;b0;b1]).
@@ -146,7 +146,7 @@ Definition double_count_by_Netlist :=
 Definition double_count_by_tb_inputs := [b14; b7; b3; b250].
 
 Definition double_count_by_tb_expected_outputs :=
-  simulate double_count_by double_count_by_tb_inputs.
+  multistep double_count_by double_count_by_tb_inputs.
 
 Definition double_count_by_tb
   := testBench "double_count_by_tb" double_count_by_interface
